cfrontend/Csem.v
@@ -351,12 +351,12 @@ Module TaggedCsem (Pol: Policy) (A: Memory ConcretePointer Pol UnitRegion) <:
     | red_const: forall v ty te m vt' ps0 ps1,
         ConstT l pct ps0 = (Success vt',ps1) ->
         rred pct (Econst v ty) te m E0 pct (Eval (v,vt') ty) te m ps0 ps1
-    | red_rvalof_mem: forall ofs pt lts bf ty te m tr v vts vt'' ps0 ps1 ps2,
-        deref_loc ty m ofs pt bf tr <<ps0>> (Success (v, vts, lts)) <<ps1>> ->
+    | red_rvalof_mem: forall p pt lts bf ty te m tr v vts vt'' ps0 ps1 ps2,
+        deref_loc ty m p pt bf tr <<ps0>> (Success (v, vts, lts)) <<ps1>> ->
         (vt <- CoalesceT l vts;;
-         vt' <- LoadT l pct pt vt lts;;
+         vt' <- LoadT l pct pt vt (concretize p) lts;;
          AccessT l pct vt') ps1 = (Success vt'',ps2) ->
-        rred pct (Evalof (Eloc (Lmem ofs pt bf) ty) ty) te m tr
+        rred pct (Evalof (Eloc (Lmem p pt bf) ty) ty) te m tr
              pct (Eval (v,vt'') ty) te m ps0 ps2
     | red_rvalof_ifun: forall b pt ty te m ps,
         rred pct (Evalof (Eloc (Lifun b pt) ty) ty) te m E0
@@ -472,14 +472,14 @@ Module TaggedCsem (Pol: Policy) (A: Memory ConcretePointer Pol UnitRegion) <:
         ConstT l pct ps0 = (Success vt',ps1) ->
         rred pct (Ealignof ty1 ty) te m E0
         pct (Eval (Vlong (Int64.repr (alignof ce ty1)), vt') ty) te m ps0 ps1
-    | red_assign_mem: forall ofs ty1 pt bf v1 vts v2 vt2 ty2 te m t1 t2 m' v'
+    | red_assign_mem: forall p ty1 pt bf v1 vts v2 vt2 ty2 te m t1 t2 m' v'
                              pct'' vt'' v'' vt''' lts lts' ps0 ps1 ps2 ps3,
         sem_cast v2 ty2 ty1 tt = Some v' ->
-        deref_loc ty1 m ofs pt bf t1 <<ps0>> (Success (v1, vts, lts)) <<ps1>> ->
+        deref_loc ty1 m p pt bf t1 <<ps0>> (Success (v1, vts, lts)) <<ps1>> ->
         ('(pct',vt') <- AssignT l pct (EffectiveT l vts) vt2;;
-        StoreT l pct' pt vt' lts) ps1 = (Success (pct'', vt'', lts'),ps2) ->
-        assign_loc ty1 m ofs pt lts' bf (v',vt'') t2 <<ps2>> (Success (m', (v'',vt'''))) <<ps3>> ->
-        rred pct (Eassign (Eloc (Lmem ofs pt bf) ty1) (Eval (v2, vt2) ty2) ty1) te m (t1++t2)
+        StoreT l pct' pt vt' (concretize p) lts) ps1 = (Success (pct'', vt'', lts'),ps2) ->
+        assign_loc ty1 m p pt lts' bf (v',vt'') t2 <<ps2>> (Success (m', (v'',vt'''))) <<ps3>> ->
+        rred pct (Eassign (Eloc (Lmem p pt bf) ty1) (Eval (v2, vt2) ty2) ty1) te m (t1++t2)
              pct'' (Eval (v'',vt''') ty1) te m' ps0 ps3
     | red_assign_tmp: forall b ty1 v1 vt1 v2 vt2 ty2 te m te' v pct' vt' ps0 ps1,
         te!b = Some (v1,vt1) ->
@@ -488,14 +488,14 @@ Module TaggedCsem (Pol: Policy) (A: Memory ConcretePointer Pol UnitRegion) <:
         AssignT l pct vt1 vt2 ps0 = (Success (pct',vt'),ps1) ->
         rred pct (Eassign (Eloc (Ltmp b) ty1) (Eval (v2, vt2) ty2) ty1) te m E0
              pct' (Eval (v,vt') ty1) te' m ps0 ps1
-    | red_assignop_mem: forall op ofs pt ty1 bf v2 vt2 ty2 tyres te m t
+    | red_assignop_mem: forall op p pt ty1 bf v2 vt2 ty2 tyres te m t
                                v1 vts vt1'' lts ps0 ps1 ps2,
-        deref_loc ty1 m ofs pt bf t <<ps0>> (Success (v1, vts, lts)) <<ps1>> ->
+        deref_loc ty1 m p pt bf t <<ps0>> (Success (v1, vts, lts)) <<ps1>> ->
         (vt1 <- CoalesceT l vts;;
-         vt1' <- LoadT l pct pt vt1 lts;;
+         vt1' <- LoadT l pct pt vt1 (concretize p) lts;;
          AccessT l pct vt1') ps1 = (Success vt1'',ps2) ->
-        rred pct (Eassignop op (Eloc (Lmem ofs pt bf) ty1) (Eval (v2,vt2) ty2) tyres ty1) te m t
-             pct (Eassign (Eloc (Lmem ofs pt bf) ty1)
+        rred pct (Eassignop op (Eloc (Lmem p pt bf) ty1) (Eval (v2,vt2) ty2) tyres ty1) te m t
+             pct (Eassign (Eloc (Lmem p pt bf) ty1)
                           (Ebinop op (Eval (v1,vt1'') ty1) (Eval (v2,vt2) ty2) tyres) ty1) te m ps0 ps2
     | red_assignop_tmp: forall op b ty1 v2 vt2 ty2 tyres te m v1 vt1 vt1' ps0 ps1,
         te!b = Some (v1,vt1) ->
@@ -513,14 +513,14 @@ Module TaggedCsem (Pol: Policy) (A: Memory ConcretePointer Pol UnitRegion) <:
              pct (Eassign (Eloc (Lefun ef tyargs tyres cc pt) ty1)
                           (Ebinop op (Eval (Vefptr ef tyargs tyres cc,pt) ty1)
                                   (Eval (v2,vt2) ty2) ty) ty1) te m ps ps
-    | red_postincr_mem: forall id ofs pt ty bf te m t v vts vt'' lts op ps0 ps1 ps2,
-        deref_loc ty m ofs pt bf t <<ps0>> (Success (v, vts, lts)) <<ps1>> ->
+    | red_postincr_mem: forall id p pt ty bf te m t v vts vt'' lts op ps0 ps1 ps2,
+        deref_loc ty m p pt bf t <<ps0>> (Success (v, vts, lts)) <<ps1>> ->
         op = match id with Incr => Oadd | Decr => Osub end ->
         (vt <- CoalesceT l vts;;
-         vt' <- LoadT l pct pt vt lts;;
+         vt' <- LoadT l pct pt vt (concretize p) lts;;
          AccessT l pct vt') ps1 = (Success vt'',ps2) ->
-        rred pct (Epostincr id (Eloc (Lmem ofs pt bf) ty) ty) te m t
-             pct (Ecomma (Eassign (Eloc (Lmem ofs pt bf) ty)
+        rred pct (Epostincr id (Eloc (Lmem p pt bf) ty) ty) te m t
+             pct (Ecomma (Eassign (Eloc (Lmem p pt bf) ty)
                                   (Ebinop op (Eval (v,vt'') ty)
                                           (Econst (Vint Int.one) type_int32s)
                                           (incrdecr_type ty))
@@ -577,12 +577,12 @@ Module TaggedCsem (Pol: Policy) (A: Memory ConcretePointer Pol UnitRegion) <:
         deref_loc ty m ofs pt bf tr <<ps0>> (Fail failure) <<ps1>> ->
         rfailred pct (Evalof (Eloc (Lmem ofs pt bf) ty) ty) te m tr failure ps0 ps1
     | failred_rvalof_mem1:
-      forall ofs pt lts bf ty te m tr v vts failure ps0 ps1 ps2,
-        deref_loc ty m ofs pt bf tr <<ps0>> (Success (v, vts, lts)) <<ps1>> ->
+      forall p pt lts bf ty te m tr v vts failure ps0 ps1 ps2,
+        deref_loc ty m p pt bf tr <<ps0>> (Success (v, vts, lts)) <<ps1>> ->
         (vt <- CoalesceT l vts;;
-        vt' <- LoadT l pct pt vt lts;;
+        vt' <- LoadT l pct pt vt (concretize p) lts;;
         AccessT l pct vt') ps1 = (Fail failure, ps2) ->
-        rfailred pct (Evalof (Eloc (Lmem ofs pt bf) ty) ty) te m tr failure ps0 ps2
+        rfailred pct (Evalof (Eloc (Lmem p pt bf) ty) ty) te m tr failure ps0 ps2
     | failred_rvalof_tmp:
       forall b ty te m v vt failure ps0 ps1,
         te!b = Some (v,vt) ->
@@ -628,20 +628,20 @@ Module TaggedCsem (Pol: Policy) (A: Memory ConcretePointer Pol UnitRegion) <:
         rfailred pct (Eassign (Eloc (Lmem ofs pt bf) ty1)
                               (Eval (v2, vt2) ty2) ty1) te m t1 failure ps0 ps1
     | failred_assign_mem1:
-      forall ofs ty1 pt bf v1 vts v2 vt2 ty2 te m t1 v' lts failure ps0 ps1 ps2,
+      forall p ty1 pt bf v1 vts v2 vt2 ty2 te m t1 v' lts failure ps0 ps1 ps2,
         sem_cast v2 ty2 ty1 tt = Some v' ->
-        deref_loc ty1 m ofs pt bf t1 <<ps0>> (Success (v1, vts, lts)) <<ps1>> ->
+        deref_loc ty1 m p pt bf t1 <<ps0>> (Success (v1, vts, lts)) <<ps1>> ->
         ('(pct',vt') <- AssignT l pct (EffectiveT l vts) vt2;;
-         StoreT l pct' pt vt' lts) ps1 = (Fail failure,ps2) ->
-        rfailred pct (Eassign (Eloc (Lmem ofs pt bf) ty1) (Eval (v2, vt2) ty2) ty1) te m t1 failure ps0 ps2
+         StoreT l pct' pt vt' (concretize p) lts) ps1 = (Fail failure,ps2) ->
+        rfailred pct (Eassign (Eloc (Lmem (concretize p) pt bf) ty1) (Eval (v2, vt2) ty2) ty1) te m t1 failure ps0 ps2
     | failred_assign_mem2:
-      forall ofs ty1 pt bf v1 vts v2 vt2 ty2 te m t1 v' lts pct'' vt'' lts' t2 failure ps0 ps1 ps2 ps3,
+      forall p ty1 pt bf v1 vts v2 vt2 ty2 te m t1 v' lts pct'' vt'' lts' t2 failure ps0 ps1 ps2 ps3,
         sem_cast v2 ty2 ty1 tt = Some v' ->
-        deref_loc ty1 m ofs pt bf t1 <<ps0>> (Success (v1, vts, lts)) <<ps1>> ->
+        deref_loc ty1 m p pt bf t1 <<ps0>> (Success (v1, vts, lts)) <<ps1>> ->
         ('(pct',vt') <- AssignT l pct (EffectiveT l vts) vt2;;
-         StoreT l pct' pt vt' lts) ps1 = (Success (pct'',vt'',lts'),ps2) ->
-        assign_loc ty1 m ofs pt lts' bf (v',vt'') t2 <<ps2>> (Fail failure) <<ps3>> ->
-        rfailred pct (Eassign (Eloc (Lmem ofs pt bf) ty1) (Eval (v2, vt2) ty2) ty1) te m (t1++t2) failure ps0 ps3
+         StoreT l pct' pt vt' (concretize p) lts) ps1 = (Success (pct'',vt'',lts'),ps2) ->
+        assign_loc ty1 m p pt lts' bf (v',vt'') t2 <<ps2>> (Fail failure) <<ps3>> ->
+        rfailred pct (Eassign (Eloc (Lmem p pt bf) ty1) (Eval (v2, vt2) ty2) ty1) te m (t1++t2) failure ps0 ps3
     | failred_assign_tmp:
       forall b ty1 v1 vt1 v2 vt2 ty2 te m v failure ps0 ps1,
         te!b = Some (v1,vt1) ->
@@ -654,12 +654,12 @@ Module TaggedCsem (Pol: Policy) (A: Memory ConcretePointer Pol UnitRegion) <:
         rfailred pct (Eassignop op (Eloc (Lmem ofs pt bf) ty1)
                                 (Eval (v2,vt2) ty2) tyres ty1) te m t1 failure ps0 ps1
     | failred_assignop_mem1:
-      forall op ofs pt ty1 bf v2 vt2 ty2 tyres te m t1 v1 vts lts failure ps0 ps1 ps2,
-        deref_loc ty1 m ofs pt bf t1 <<ps0>> (Success (v1,vts, lts)) <<ps1>> ->
+      forall op p pt ty1 bf v2 vt2 ty2 tyres te m t1 v1 vts lts failure ps0 ps1 ps2,
+        deref_loc ty1 m p pt bf t1 <<ps0>> (Success (v1,vts, lts)) <<ps1>> ->
         (vt1 <- CoalesceT l vts;;
-         vt1' <- LoadT l pct pt vt1 lts;;
+         vt1' <- LoadT l pct pt vt1 (concretize p) lts;;
          AccessT l pct vt1') ps1 = (Fail failure,ps2) ->
-        rfailred pct (Eassignop op (Eloc (Lmem ofs pt bf) ty1)
+        rfailred pct (Eassignop op (Eloc (Lmem p pt bf) ty1)
                                 (Eval (v2,vt2) ty2) tyres ty1) te m t1 failure ps0 ps2
     | failred_assignop_tmp:
       forall op b ty1 v2 vt2 ty2 tyres te m v1 vt1 failure ps0 ps1,
@@ -671,12 +671,12 @@ Module TaggedCsem (Pol: Policy) (A: Memory ConcretePointer Pol UnitRegion) <:
         deref_loc ty m ofs pt bf tr <<ps0>> (Fail failure) <<ps1>> ->
         rfailred pct (Epostincr id (Eloc (Lmem ofs pt bf) ty) ty) te m tr failure ps0 ps1
     | failred_postincr_mem1:
-      forall id ofs pt ty bf te m tr v vts lts failure ps0 ps1 ps2,
-        deref_loc ty m ofs pt bf tr <<ps0>> (Success (v,vts, lts)) <<ps1>> ->
+      forall id p pt ty bf te m tr v vts lts failure ps0 ps1 ps2,
+        deref_loc ty m p pt bf tr <<ps0>> (Success (v,vts, lts)) <<ps1>> ->
         (vt <- CoalesceT l vts;;
-         vt' <- LoadT l pct pt vt lts;;
+         vt' <- LoadT l pct pt vt (concretize p) lts;;
          AccessT l pct vt') ps1 = (Fail failure,ps2) ->
-        rfailred pct (Epostincr id (Eloc (Lmem ofs pt bf) ty) ty) te m tr failure ps0 ps2
+        rfailred pct (Epostincr id (Eloc (Lmem p pt bf) ty) ty) te m tr failure ps0 ps2
     | failred_postincr_tmp:
       forall id b ty te m v vt failure ps0 ps1,
         te!b = Some (v,vt) ->
